examples/school2014/exercises/ex9d-padding.fst
@@ -1,0 +1,34 @@
+module Pad
+open Array
+
+(* a coercion; avoid it? *)
+assume val n2b: n:nat {( n < 256 )} -> Tot uint8
+assume val b2n: b:uint8 -> Tot (n:nat { (n < 256) /\ n2b n = b })
+
+type bytes = seq byte (* concrete byte arrays *) 
+type nbytes (n:nat) = b:bytes{length b == n} (* fixed-length bytes *)
+
+let blocksize = 32 
+type block = nbytes blocksize
+type text = b:bytes {(length b < blocksize)}
+
+(* fill in type here *)
+let pad n = 
+  Array.create n (n2b (n-1))  
+
+(* pad 1 = [| 0 |]; pad 2 = [| 1; 1 |]; ... *)
+
+(* fill in type here *)
+let encode a = append a (pad (blocksize - length a))
+
+(* fill in type here *)
+let decode (b:block) = 
+  let padsize = b2n(index b (blocksize - 1)) + 1 in
+  if op_LessThan padsize blocksize then 
+    let (plain,padding) = split b (blocksize - padsize) in
+    if padding = pad padsize
+    then Some plain
+    else None   
+  else None
+
+
