examples/school2014/solutions/ex9bc-rpc.fst
@@ -2,8 +2,8 @@
 
 module RPC
 open Array
-open Format
 open SHA1
+open Format
 open MAC
 
 (* some basic, untrusted network controlled by the adversary *)
@@ -16,23 +16,23 @@ assume val recv: (message -> unit) -> unit
 logic type Request : string -> Type
 logic type Response : string -> string -> Type
 
-(* let k = keygen (fun msg -> (exists s. msg = request s /\ Request s) \/       *)
-(*                            (exists s t. msg = response s t /\ Response s t)) *)
-opaque logic type reqresp (msg:message) =
-    (exists s. msg = request s /\ Request s)
-      \/ (exists s t. msg = response s t /\ Response s t)
+(* the meaning of MACs, as used in RPC *)
 
-assume val k : pkey reqresp
+opaque logic type reqresp (msg:message) =
+    (exists s.   msg = Format.request s    /\ Request s)
+ \/ (exists s t. msg = Format.response s t /\ Response s t)
+
+let k = keygen reqresp 
 
 let client (s:string16) =
   assume (Request s);
-  send (append (utf8 s) (mac k (request s))); 
+  send (append (utf8 s) (mac k (Format.request s))); 
   recv (fun msg ->
     if length msg < macsize then failwith "Too short"
     else
       let (v, m') = split msg (length msg - macsize) in
       let t = iutf8 v in
-      if verify k (response s t) m'
+      if verify k (Format.response s t) m'
       then assert (Response s t))
 
 let server () =
@@ -43,12 +43,12 @@ let server () =
       if length v > 65535 then failwith "Too long" 
       else
         let s = iutf8 v in
-        if verify k (request s) m 
+        if verify k (Format.request s) m 
         then  
           ( assert (Request s);
             let t = "22" in
             assume (Response s t);
-            send (append (utf8 t) (mac k (response s t)))))
+            send (append (utf8 t) (mac k (Format.response s t)))))
   
 (* 
 let test () = 
